MergeSort stucked

MergeSort.dfy
@@ -12,7 +12,7 @@ predicate SortedSequence(q: seq<int>)
 predicate isLeftArr(a: array<int>, left: array<int>, middle: nat)
 	reads left, a
 {
-	a.Length >= 2 && middle == a.Length / 2 && 0 < middle < a.Length &&
+	a.Length >= 2 && middle == (a.Length - 1) / 2 && 0 < middle < a.Length &&
 	left.Length == middle + 1 &&
 	forall j :: 0 <= j < middle + 1 < left.Length ==> left[j] == a[j]
 }
@@ -20,7 +20,7 @@ predicate isLeftArr(a: array<int>, left: array<int>, middle: nat)
 predicate isRightArr(a: array<int>, right: array<int>, middle: nat)
 	reads right, a
 {
-	a.Length >= 2 && middle == a.Length / 2 && 0 < middle < a.Length &&
+	a.Length >= 2 && middle == (a.Length - 1) / 2 && 0 < middle < a.Length &&
 	right.Length == a.Length - (middle + 1) &&
 	forall j :: 0 <= j < (a.Length - (middle + 1)) < right.Length  ==> right[j] == a[j + (middle + 1)]
 }
@@ -31,7 +31,7 @@ predicate isSorted(origin: array<int>, sortedArr: array<int>)
 	sortedArr.Length == origin.Length && Sorted(sortedArr) && multiset(origin[..]) == multiset(sortedArr[..])
 }
 
-method MergeSort(a: array<int>) returns (b: array<int>)
+method {:verify false} MergeSort(a: array<int>) returns (b: array<int>)
 	ensures b.Length == a.Length && Sorted(b) && multiset(a[..]) == multiset(b[..])
 	decreases a.Length
 	{
@@ -42,7 +42,7 @@ method MergeSort(a: array<int>) returns (b: array<int>)
 		}
 	}
 
-method Assign1 (a: array<int>) returns (b: array<int>)
+method {:verify false} Assign1 (a: array<int>) returns (b: array<int>)
 	requires a.Length < 2
 	ensures b.Length == a.Length && Sorted(b) && multiset(a[..]) == multiset(b[..])
 {
@@ -56,7 +56,7 @@ lemma LemmaS1 (a: array<int>)
 
 {}
 
-method MergeSort1 (a: array<int>) returns (b: array<int>)
+method {:verify false} MergeSort1 (a: array<int>) returns (b: array<int>)
 	requires a.Length >= 2
 	ensures b.Length == a.Length && Sorted(b) && multiset(a[..]) == multiset(b[..])
 {
@@ -66,9 +66,9 @@ method MergeSort1 (a: array<int>) returns (b: array<int>)
 
 }
 
-method MergeSort2 (a: array<int>, middle: nat) returns (b: array<int>) 
+method {:verify false} MergeSort2 (a: array<int>, middle: nat) returns (b: array<int>) 
 	requires a.Length >= 2
-	requires middle == a.Length / 2 && 0 < middle < a.Length
+	requires middle == (a.Length - 1) / 2 && 0 < middle < a.Length
 	ensures b.Length == a.Length && Sorted(b) && multiset(a[..]) == multiset(b[..])
 {
 	// Sequential Composition
@@ -76,23 +76,22 @@ method MergeSort2 (a: array<int>, middle: nat) returns (b: array<int>)
 	b := MergeSort3(a, left, right, middle);
 }
 
-method AssignMiddle (a: array<int>) returns (m: nat) 
+method {:verify false} AssignMiddle (a: array<int>) returns (m: nat) 
 	requires a.Length >= 2
-	ensures m == a.Length / 2 && 0 < m < a.Length
+	ensures m == (a.Length - 1) / 2 && 0 <= m < a.Length
 {
 	LemmaS2(a);
-	m := a.Length / 2;
+	m := (a.Length - 1) / 2;
 }
 
 lemma LemmaS2 (a: array<int>) 
 	requires a.Length >= 2
-	ensures a.Length / 2 == a.Length / 2 && 0 < a.Length / 2 < a.Length 
-{
-}
+	ensures (a.Length - 1) / 2 == (a.Length - 1) / 2 && 0 <= (a.Length - 1) / 2 < a.Length 
+{}
 
 
-method Assign3Split(a: array<int>, middle: nat) returns (left: array<int>, right: array<int>) 
-	requires a.Length >= 2 && middle == a.Length / 2 && 0 < middle < a.Length
+method {:verify false} Assign3Split (a: array<int>, middle: nat) returns (left: array<int>, right: array<int>)
+	requires a.Length >= 2 && middle == (a.Length - 1) / 2 && 0 <= middle < a.Length
 	ensures isLeftArr(a, left, middle)
 	ensures isRightArr(a, right, middle)
 {
@@ -100,8 +99,8 @@ method Assign3Split(a: array<int>, middle: nat) returns (left: array<int>, right
 	right :=  Assign3Right(a, middle);
 }
 
-method Assign3Left(a: array<int>, middle: nat) returns (arr: array<int>) 
-	requires a.Length >= 2 && middle == a.Length / 2 && 0 < middle < a.Length
+method {:verify false} Assign3Left(a: array<int>, middle: nat) returns (arr: array<int>) 
+	requires a.Length >= 2 && middle == (a.Length - 1) / 2 && 0 <= middle < a.Length
 	ensures isLeftArr(a, arr, middle)
 {
 	var i := 0;
@@ -117,8 +116,8 @@ method Assign3Left(a: array<int>, middle: nat) returns (arr: array<int>)
 	}
 } 
 
-method LeftLoopBody(arr: array<int>, a: array<int>, i: nat, middle: nat) 
-	requires a.Length >= 2 && middle == a.Length / 2 && middle > 0 // Pre
+method {:verify true} LeftLoopBody(arr: array<int>, a: array<int>, i: nat, middle: nat) 
+	requires a.Length >= 2 && middle == (a.Length - 1) / 2 && middle >= 0 // Pre
 	requires arr.Length == middle + 1
 	requires i < middle + 1 && forall j :: 0 <= j < i < arr.Length ==> arr[j] == a[j]
 	ensures forall j :: 0 <= j < i + 1  < arr.Length ==> arr[j] == a[j] // post cond of following assignment
@@ -129,14 +128,14 @@ method LeftLoopBody(arr: array<int>, a: array<int>, i: nat, middle: nat)
 } 
 
 lemma  LemmaArrI(arr: array<int>, a: array<int>, i: nat, middle: nat, ai: int)
-	requires a.Length >= 2 && middle == a.Length / 2 && middle > 0 // Pre
-	requires arr.Length == middle + 1 >= 2
+	requires a.Length >= 2 && middle == (a.Length - 1) / 2 && middle >= 0 // Pre
+	requires arr.Length == middle + 1 >= 1
 	requires i < middle + 1 && forall j :: 0 <= j < i < arr.Length ==> arr[j] == a[j]
 	requires ai == a[i]
 	ensures arr[..i] + [ai] == a[..i+1]
 {}
-method Assign3Right(a: array<int>, middle: nat) returns (arr: array<int>) 
-	requires a.Length >= 2 && middle == a.Length / 2 && 0 < middle < a.Length
+method {:verify true}  Assign3Right(a: array<int>, middle: nat) returns (arr: array<int>) 
+	requires a.Length >= 2 && middle == (a.Length - 1) / 2 && 0 < middle < a.Length
 	ensures isRightArr(a, arr, middle)
 {
 	var i := 0;
@@ -152,8 +151,8 @@ method Assign3Right(a: array<int>, middle: nat) returns (arr: array<int>)
 	}
 } 
 
-method RightLoopBody(arr: array<int>, a: array<int>, i: nat, middle: nat) 
-	requires a.Length >= 2 && middle == a.Length / 2 && 0 < middle < a.Length // Pre
+method {:verify true}  RightLoopBody(arr: array<int>, a: array<int>, i: nat, middle: nat) 
+	requires a.Length >= 2 && middle == (a.Length - 1) / 2 && 0 <= middle < a.Length // Pre
 	requires 0 <= i < a.Length - (middle + 1) // Guard
 	requires forall j :: 0 <= j < i < arr.Length ==> arr[j] == a[j + middle + 1] // Inv
 	requires arr.Length == a.Length - (middle + 1)
@@ -165,34 +164,33 @@ method RightLoopBody(arr: array<int>, a: array<int>, i: nat, middle: nat)
 } 
 
 lemma LemmaArrIRight(arr: array<int>, a: array<int>, i: nat, middle: nat, ai: int)
-	requires a.Length >= 2 && middle == a.Length / 2 && 0 < middle < a.Length // Pre
+	requires a.Length >= 2 && middle == (a.Length - 1) / 2 && 0 <= middle < a.Length // Pre
 	requires 0 <= i < a.Length - (middle + 1) // Guard
 	requires ai == a[i + middle + 1] && arr.Length == a.Length - (middle + 1)
 	requires forall j :: 0 <= j < i < arr.Length ==> arr[j] == a[j + middle + 1] // Inv
 	ensures arr[..i] + [ai] == a[middle+1 .. (i + middle + 2)]
 {}
 
-method MergeSort3(a: array<int>, left: array<int>, right: array<int>, middle: nat) returns(b: array<int>)
+method {:verify true}  MergeSort3(a: array<int>, left: array<int>, right: array<int>, middle: nat) returns(b: array<int>)
 	requires isLeftArr(a, left, middle) && isRightArr(a, right, middle)
 	ensures b.Length == a.Length && Sorted(b) && multiset(a[..]) == multiset(b[..])
 {
-	b := new int[a.Length];
 	//Sequantion composition
 	var sortedL, sortedR := MergeSort3a(a, left, right, middle);
-	b := MergeSort3b(b, left, right,sortedL, sortedR, middle);
+	b := MergeSort3b(a, left, right,sortedL, sortedR, middle);
 }
 
-method MergeSort3a(a: array<int>, left: array<int>, right: array<int>, middle: nat) returns(sortedL: array<int>, sortedR: array<int>)
+method {:verify true}  MergeSort3a(a: array<int>, left: array<int>, right: array<int>, middle: nat) returns(sortedL: array<int>, sortedR: array<int>)
 	requires isLeftArr(a, left, middle) && isRightArr(a, right, middle)
 	ensures isSorted(left, sortedL) && isSorted(right, sortedR)
 	
 {
 	//Sequantion composition
-	// sortedL := MergeSort(left);
-	// sortedR := MergeSort(right);
+	sortedL := MergeSort(left);
+	sortedR := MergeSort(right);
 }
 
-method MergeSort3b(a: array<int>, left: array<int>, right: array<int>,sortedL: array<int>, sortedR: array<int>, middle: nat) returns(b: array<int>)
+method {:verify true}  MergeSort3b(a: array<int>, left: array<int>, right: array<int>,sortedL: array<int>, sortedR: array<int>, middle: nat) returns(b: array<int>)
 	requires isLeftArr(a, left, middle) && isRightArr(a, right, middle)
 	requires isSorted(left, sortedL) && isSorted(right, sortedR)
 	{
@@ -201,7 +199,7 @@ method MergeSort3b(a: array<int>, left: array<int>, right: array<int>,sortedL: a
 	}
 
 
-method Merge(b: array<int>, c: array<int>, d: array<int>)
+method {:verify true}  Merge(b: array<int>, c: array<int>, d: array<int>)
 	requires b != c && b != d && b.Length == c.Length + d.Length
 	requires Sorted(c) && Sorted(d)
 	ensures Sorted(b) && multiset(b[..]) == multiset(c[..])+multiset(d[..])
@@ -209,28 +207,218 @@ method Merge(b: array<int>, c: array<int>, d: array<int>)
 	{
 		var k,l,r := 0,0,0;
 		k,l,r := MergeWhileLoop(b, c, d, k, l, r);
-		
+		assert ((l == c.Length && r < d.Length) || (l < c.Length && r == d.Length));
+		MergeRest(b, c, d, k, l, r);
 	}
-method MergeWhileLoop(b: array<int>, c: array<int>, d: array<int>, k0: nat, l0: nat, r0: nat) returns(k: nat, l: nat, r: nat)
+
+predicate CrossSorted(b: array<int>, c: array<int>, d: array<int>, k: nat, l: nat, r: nat) 
+	reads b, c, d
+{
+	forall i, n, m :: (0 <= i < k < b.Length && l <= n < c.Length && r <= m < d.Length) ==> b[i] <= c[n] && b[i] <= d[m] // Sorted(b[.. k])
+}
+predicate MergeInv(b: array<int>, c: array<int>, d: array<int>, k: nat, l: nat, r: nat) 
+	reads b, c, d
+{
+	 0 <= k <= b.Length && 0 <= l <= c.Length && 0 <= r <= d.Length &&  k == l + r && 
+	 multiset(b[..k]) == multiset(c[..l] + d[..r]) && CrossSorted(b,c,d,k,l,r) &&
+	 forall i,j :: 0 <= j < i < k ==> b[j] <= b[i] // Sorted(b[.. k])
+}
+
+predicate areValidIndices (b: array<int>, c: array<int>, d: array<int>, k: int, l: int, r: int) 
+{
+	0 <= k < b.Length && 0 <= l < c.Length && 0 <= r < d.Length 	
+}
+method {:verify false}  MergeWhileLoop(b: array<int>, c: array<int>, d: array<int>, k0: nat, l0: nat, r0: nat) returns(k: nat, l: nat, r: nat)
+	requires b != c && b != d && b.Length == c.Length + d.Length
+	requires Sorted(c) && Sorted(d) 
+	requires k0 == 0 && l0 == 0 && r0 == 0
+	ensures MergeInv(b,c,d,k,l,r) 
+	ensures (l == c.Length && r < d.Length) || (l < c.Length && r == d.Length)
+	modifies b
+{
+	k, l, r := k0, l0, r0;
+	while (r < d.Length && l < c.Length && k < b.Length)
+		decreases b.Length - k
+		invariant MergeInv(b,c,d,k,l,r)
+	{
+		// Following Assignment k
+		k,l,r := MergeLoopBody(b, c, d, k, l, r);
+		k := k + 1;
+	}
+}
+
+method {:verify false} MergeLoopBody(b: array<int>, c: array<int>, d: array<int>, k0: nat, l0: nat, r0: nat) returns(k: nat, l: nat, r: nat)
+	requires b != c && b != d && b.Length == c.Length + d.Length
+	requires Sorted(c) && Sorted(d) 
+	requires MergeInv(b,c,d,k0,l0,r0) && k0 < b.Length && l0 < c.Length && r0 < d.Length  // Inv & Guard
+	ensures MergeInv(b,c,d,k+1,l,r) && 0 <= l <= c.Length && r0 + l0 < r + l
+{
+	k, l, r := k0, l0, r0;
+	if (c[l] <= d[r]) {
+		// Following Assignment l
+		MergeLoopBody1(b,c,d,k,l,r);
+		l := l+1;
+	} else {
+		// Following Assignment r
+		MergeLoopBody2(b,c,d,k,l,r);
+		r := r+1;
+	}
+}
+
+method {:verify true}  MergeLoopBody1(b: array<int>, c: array<int>, d: array<int>, k0: nat, l0: nat, r0: nat) 
+	requires b != c && b != d && b.Length == c.Length + d.Length
+	requires Sorted(c) && Sorted(d) 
+	requires MergeInv(b,c,d,k0,l0,r0) && k0 < b.Length && l0 < c.Length && r0 < d.Length  // Inv & Guard
+	requires c[l0] <= d[r0] // If Test
+	ensures MergeInv(b,c,d,k0+1,l0+1,r0)
+	modifies b
+{
+	// Following assignment k0+1
+	LemmaLB1(b,c,d,k0+1,l0+1,r0);
+	b[k0] := c[l0];
+}
+
+lemma LemmaLB1(b: array<int>, c: array<int>, d: array<int>, k: nat, l: nat, r: nat)
+	requires b != c && b != d && b.Length == c.Length + d.Length
+	requires Sorted(c) && Sorted(d) 
+	requires areValidIndices(b,c,d,k-1,l-1,r) && MergeInv(b,c,d,k-1,l-1,r) 
+	requires c[l-1] <= d[r] // If Test
+	// Modify MergeInv
+	ensures 0 <= k <= b.Length && 0 <= l <= c.Length && 0 <= r <= d.Length &&  k == l + r && 
+	 multiset(b[..k-1] + [c[l-1]]) == multiset(c[..l] + d[..r]) && 
+	 forall i, n, m :: (0 <= i < k - 1 < b.Length && l <= n < c.Length && r <= m < d.Length) ==> b[i] <= c[n] && b[i] <= d[m] && c[l-1] <= d[m] // Sorted(b[.. k])  
+	ensures forall i,j :: 0 <= j < i < k - 1 ==> b[j] <= b[i] && b[j] <= c[l-1] // Sorted(b[.. k])
+{}
+
+method {:verify true}  MergeLoopBody2(b: array<int>, c: array<int>, d: array<int>, k0: nat, l0: nat, r0: nat) 
+	requires b != c && b != d && b.Length == c.Length + d.Length
+	requires Sorted(c) && Sorted(d) 
+	requires MergeInv(b,c,d,k0,l0,r0) && k0 < b.Length && l0 < c.Length && r0 < d.Length  // Inv & Guard
+	requires c[l0] > d[r0] // !If Test
+	ensures MergeInv(b,c,d,k0+1,l0,r0+1)
+	modifies b
+{
+	// Following assignment k0+1
+	LemmaLB2(b,c,d,k0+1,l0,r0+1);
+	b[k0] := d[r0];
+}
+
+lemma LemmaLB2(b: array<int>, c: array<int>, d: array<int>, k: nat, l: nat, r: nat)
+	requires b != c && b != d && b.Length == c.Length + d.Length
+	requires Sorted(c) && Sorted(d) 
+	requires areValidIndices(b,c,d,k-1,l,r-1) && MergeInv(b,c,d,k-1,l,r-1) 
+	requires c[l] > d[r-1] // !If Test
+	// Modify MergeInv
+	ensures 0 <= k <= b.Length && 0 <= l <= c.Length && 0 <= r <= d.Length &&  k == l + r && 
+	 multiset(b[..k-1] + [d[r-1]]) == multiset(c[..l] + d[..r]) && 
+	 forall i, n, m :: (0 <= i < k - 1 < b.Length && l <= n < c.Length && r <= m < d.Length) ==> b[i] <= c[n] && b[i] <= d[m] && d[r-1] <= c[n] // Sorted(b[.. k])  
+	ensures forall i,j :: 0 <= j < i < k - 1 ==> b[j] <= b[i] && b[j] <= d[r-1] // Sorted(b[.. k])
+{}
+
+method {:verify true}  MergeRest(b: array<int>, c: array<int>, d: array<int>, k: nat, l: nat, r: nat)
 	requires b != c && b != d && b.Length == c.Length + d.Length
 	requires Sorted(c) && Sorted(d)
-	ensures 0 <= k < b.Length && 0 <= l < c.Length && 0 <= r < d.Length
-	ensures forall i,j :: 0 <= j < i < k ==> b[j] <= b[i] // Sorted(b[.. k])
-	ensures multiset(b[..k]) == multiset(c[..l] + d[..r])
+	requires MergeInv(b,c,d,k,l,r) && ((l == c.Length && r < d.Length) || (l < c.Length && r == d.Length))
+	ensures Sorted(b) && multiset(b[..]) == multiset(c[..])+multiset(d[..])
+	modifies b 
+{
+	if (l == c.Length) {
+		MergeRest1(b,c,d,k,l,r);
+	} else {
+		MergeRest2(b,c,d,k,l,r);
+	}
+}
+
+predicate MergeRestInv(b: array<int>, c: array<int>, d: array<int>, k: nat, l: nat, r: nat) 
+	reads b, c, d
+{
+	 0 <= k <= b.Length && 0 <= l <= c.Length && 0 <= r <= d.Length &&  k == l + r && 
+	 multiset(b[..k]) == multiset(c[..l] + d[..r]) && 
+	 forall i,j :: 0 <= j < i < k ==> b[j] <= b[i] // Sorted(b[.. k])
+}
+
+predicate CrossSortedRest1(b: array<int>, arr: array<int>, k: nat, index: nat) 
+	reads b, arr
+{
+	forall i, n :: (0 <= i < k < b.Length && index <= n < arr.Length ) ==> b[i] <= arr[n] // Sorted(b[.. k])
+}
+method {:verify true}  MergeRest1(b: array<int>, c: array<int>, d: array<int>, k: nat, l: nat, r: nat)
+	requires b != c && b != d && b.Length == c.Length + d.Length
+	requires Sorted(c) && Sorted(d)
+	requires MergeInv(b,c,d,k,l,r)
+	requires forall j, m :: 0 <= j < k && r <= m < d.Length ==> b[j] <= d[m]
+	requires ((l == c.Length && r < d.Length) || (l < c.Length && r == d.Length)) && l == c.Length//r < d.Length // Guard
+	ensures Sorted(b) && multiset(b[..]) == multiset(c[..])+multiset(d[..]) 
 	modifies b
-	{}
+{
+	var r1: nat, k1: nat := r, k;
+	assert r1 < d.Length;
+	assert 	forall i, n, m :: (0 <= i < k < b.Length && l <= n < c.Length && r <= m < d.Length) ==> b[i] <= c[n] && b[i] <= d[m]; // Sorted(b[.. k])
+
+	while (k1 < b.Length && r1 < d.Length) 
+		decreases b.Length - k1
+		invariant MergeRestInv(b,c,d,k1,l,r1) 
+	{
+		assert 	forall i, n, m :: (0 <= i < k < b.Length && l <= n < c.Length && r <= m < d.Length) ==> b[i] <= c[n] && b[i] <= d[m]; // Sorted(b[.. k])
+
+		assert MergeRestInv(b,c,d,k1,l,r1);
+
+		assert r1 < d.Length;
+		b[k1] := d[r1];
+		r1 := r1 + 1;
+		k1 := k1 + 1;
+
+
+		assert 0 <= k1 <= b.Length;
+		assert 0 <= l <= c.Length;
+		assert 0 <= r1 <= d.Length;
+		assert  k1 == l + r1;
+	 	assert multiset(b[..k1]) == multiset(c[..l] + d[..r1]);
+	 	assert forall i,j :: 0 <= j < i < k1 < b.Length ==> b[j] <= b[i]; // Sorted(b[.. k])
+	}
+}
+
+method {:verify true}  MergeRest2(b: array<int>, c: array<int>, d: array<int>, k: nat, l: nat, r: nat)
+	requires b != c && b != d && b.Length == c.Length + d.Length
+	requires Sorted(c) && Sorted(d)
+	requires MergeInv(b,c,d,k,l,r)
+	requires l < c.Length // Guard
+	ensures Sorted(b) && multiset(b[..]) == multiset(c[..])+multiset(d[..]) 
+	modifies b
+{
+	var l1: nat, k1: nat := l, k;
+	assert l1 < d.Length;
+	while (k1 < b.Length && l1 < c.Length) 
+		decreases b.Length - k1
+		invariant MergeRestInv(b,c,d,k1,l1,r) 
+	{
+		b[k1] := c[l1];
+		l1 := l1 + 1;
+		k1 := k1 + 1;
+		// assert 0 <= k1 <= b.Length;
+		// assert 0 <= l <= c.Length;
+		// assert 0 <= r1 <= d.Length;
+		// assert  k1 == l + r1;
+	 	// assert multiset(b[..k1]) == multiset(c[..l] + d[..r1]);
+	}
+}
 
 method Main() {
-	var a := new int[3];
-	a[0], a[1], a[2] := 4, 8, 6;
+	var a := new int[6];
+	a[0] := 10;
+	a[1] := 39;
+	a[2] := 1;
+	a[3] := 0;
+	a[4] := -1;
+	a[5] := 2;
 	var q0 := a[..];
-	assert q0 == [4,8,6];
+	// assert q0 == [4,8,6];
 	a := MergeSort(a);
-	assert a.Length == |q0| && multiset(a[..]) == multiset(q0);
+	// assert a.Length == |q0| && multiset(a[..]) == multiset(q0);
 	print "the sorted version of [4, 8, 6] is ";
 	print a[..];
-	assert Sorted(a);
-	assert a[..] == [4,6,8];
+	// assert Sorted(a);
+	// assert a[..] == [4,6,8];
 }
 
 
